theories/wp_tactics.v
@@ -31,15 +31,43 @@ Ltac wp_simplify :=
   repeat progress (wp_decide; cbn);
   try rewrite !fold_bind.
 
+(* Simplify goals that introduce simple values. *)
+
+Ltac wp_intro :=
+  match goal with |- ∀ v, v = VUnit → _ => intros v ?; subst v end.
+
+(* Deal with a goal of the form [safe (if b then ok else _)]. *)
+
+Ltac wp_scoped_case_analysis :=
+  match goal with |- safe (if ?b then Ret VUnit else _) _ =>
+    (* We wish to perform a case analysis on [b], but first, we must
+       limit the scope of this case analysis by claiming that this
+       runtime assertion always succeeds. *)
+    eapply safe_covariant with (φ := λ v, v = VUnit);
+    [ destruct b; [
+        (* trivial goal here: [VUnit = VUnit] *)
+        wp_step; apply eq_refl
+      | (* user goal here: must prove that the assertion succeeds *)
+        idtac
+      ]
+    | wp_intro (* user goal here: continuation *) ]
+  end
+
 (* Reduce and reason about a goal of the form [safe m φ]. *)
 
-Ltac wp :=
-  unfold wp;
-  (* Repeatedly simplify. *)
-  wp_simplify;
-  repeat first [
+with wp_step :=
+  first [
     apply prove_safe_ret; wp_simplify
   | apply prove_safe_bind; wp_simplify
   | apply prove_safe_stop; wp_simplify
   | apply prove_safe_flip; intro; wp_simplify
+  | wp_scoped_case_analysis
   ].
+
+(* Apply brute force. *)
+
+Ltac wp :=
+  unfold wp;
+  wp_simplify;
+  repeat wp_step.
+    (* TODO not clearly correct: should we iterate? *)
